\documentclass{article}
\usepackage{amsmath}
\usepackage{amssymb}
\usepackage{amsthm}
\usepackage{cancel}
\usepackage[utf8]{inputenc}
\usepackage[english]{babel}
\usepackage{color}

\newtheorem{theorem}{Theorem}
\begin{document}

\title{Finding correlation for acmPRS}

\maketitle

\textbf{Goals:}

\begin{itemize}
	\item Find $Var(\text{acmPRS})$
	\item Find $Cov(Y, \text{acmPRS})$
\end{itemize}

\subsection{Finding $Var(\text{acmPRS})$:}

Define 
$$ 
\begin{aligned} 
\hat{S}_i &= \sum^{m_i}_{j = 1} \hat{\beta} \mathbf{G_j} \\
\hat{S}_{acm} &= \sum^c_{i=1} n_i r_i \sqrt{\frac{h_i}{h_1}} \hat{S}_i 
\end{aligned} 
$$



\begin{theorem}
$E[\hat{S}_{acm}] = 0$ 
\end{theorem}

\begin{proof}
$$ 
\begin{aligned}
E[\hat{S}_{acm}] &= E[\sum^c_{i=1} n_i r_i \sqrt{\frac{h_i}{h_1}} \hat{S}_i] \\
&= \sum^c_{i=1} E[n_i r_i \sqrt{\frac{h_i}{h_1}} \hat{S}_i] \\
&= \sum^c_{i=1} n_i r_i \sqrt{\frac{h_i}{h_1}} E[\hat{S}_i] \\ \\
&\because E[\hat{S}_i] = 0 \\
&\therefore E[\hat{S}_{acm}] = 0
\end{aligned}
$$
\end{proof}

\newpage

\begin{theorem}
$Var(\hat{S}_{acm}) =\sum^c_{i=1}  \frac{m_i n^2_i r^2_i h_i}{h_1}  Var(\hat{\beta}_i) +  \sum^c_{i \neq j} n_i n_j r_i r_j \sqrt{\frac{h_i h_j}{h^2_1}} Cov(\hat{S}_i, \hat{S}_j)]$
\end{theorem}

\begin{proof}

$$
\begin{aligned}
Var(\sum^c_{i=1} n_i r_i \sqrt{\frac{h_i}{h_1}} \hat{S}_i) &= \sum^c_{i=1} Var \left( n_i r_i \sqrt{\frac{h_i}{h_1}} \hat{S}_i \right) + \sum_{i \neq j} Cov \left( n_i r_i \sqrt{\frac{h_i}{h_1}} \hat{S}_i, n_j r_j \sqrt{\frac{h_j}{h_1}} \hat{S}_j \right) 
\end{aligned}
$$

\begin{equation}
\begin{aligned}
\sum^c_{i=1} Var \left( n_i r_i \sqrt{\frac{h_i}{h_1}} \hat{S}_i \right) &= \sum^c_{i=1} n_i r_i \sqrt{\frac{h_i}{h_1}}  Var(\hat{S}_i) \\
&= \sum^c_{i=1} n_i r_i \sqrt{\frac{h_i}{h_1}} m_i Var(\hat{\beta}_i)      \\
\end{aligned}
\end{equation}

\begin{equation}
\begin{aligned}
\sum_{i \neq j} Cov \left(  n_i r_i \sqrt{\frac{h_i}{h_1}} \hat{S}_i,  n_j r_j \sqrt{\frac{h_j}{h_1}} \hat{S}_j \right) &= \scriptstyle \sum_{i \neq j} E \left[ \left( n_i r_i \sqrt{\frac{h_i}{h_1}} \hat{S}_i \right), \left( n_j r_j \sqrt{\frac{h_j}{h_1}} \hat{S}_j  \right)  \right] + \scriptscriptstyle \cancelto{0}{E \left[ \sum^c_{i=1} n_i r_i \sqrt{\frac{h_i}{h_1}}] \hat{S}_i \right]} \cancelto{0}{E \left[ \sum^c_{j=1} n_j r_j \sqrt{\frac{h_j}{h_1}} \hat{S}_j \right]} \\
&= \sum_{i \neq j} n_i n_j r_i r_j \sqrt{\frac{h_i h_j}{h^2_1}} E[\hat{S}_i \hat{S}_j]\\ 
&= \sum_{i \neq j} n_i n_j r_i r_j \sqrt{\frac{h_i h_j}{h^2_1}} Cov \left( \hat{S}_i, \hat{S}_j \right) \\ 
\end{aligned}
\end{equation}


The above is because

$$
\begin{aligned}
Cov( \hat{S}_i, \hat{S}_j) &= E \left[ \hat{S}_i \hat{S}_j \right] + \cancelto{0}{E[ \hat{S}_i]} + \cancelto{0}{E[ \hat{S}_j ]} \\
&=  E \left[ \hat{S}_i \hat{S}_j \right]
\end{aligned}
$$

Combining (1) and (2): 

$$ Var(\hat{S}_{acm}) =\sum^c_{i=1}  \frac{m_i n^2_i r^2_i h_i}{h_1}  Var(\hat{\beta}_i) +  \sum^c_{i \neq j} n_i n_j r_i r_j \sqrt{\frac{h_i h_j}{h^2_1}} Cov(\hat{S}_i, \hat{S}_j)] $$

\end{proof}

\newpage

\begin{theorem}
$Cov(Y, \text{acmPRS}) = \frac{1}{c} \sum^c_{i=1} n_i r_i \sqrt{\frac{h_i}{h_1}} m_i Cov(\hat{\beta}_i, \beta_{Y})$
\end{theorem}

\begin{proof}

$$
\begin{aligned}
\text{Cov}(Y, \text{acmPRS}) &= E[Y \text{acmPRS}] + \cancelto{0}{E[Y]} + \cancelto{0}{E[\text{acmPRS}]} \\
&= E \left[ \left( \sum^m_{j=1} \beta_{j Y} G_i \right) \left( \sum^c_{i=1} n_i r_i \sqrt{\frac{h_i}{h_1}} \sum^m_{j=1} \hat{\beta}_{j i} G_j \right) \right] 
\end{aligned}
$$   

\textcolor{red}{I'm really not sure if I'm allowed to do this.}

$$ 
\begin{aligned}
E \left[ \left( \sum^m_{j=1} \beta_{j Y} G_i \right) \left( \sum^c_{i=1} n_i r_i \sqrt{\frac{h_i}{h_1}} \sum^m_{j=1} \hat{\beta}_{j i} G_j \right) \right] &= E \left[ \sum^c_{i=1} n_i r_i \sqrt{\frac{h_i}{h_1}} \left[ \sum^{m_i} \beta_j G_j \right] \frac{1}{c} \left[ \sum^{m_Y} \beta_{jY} G_j \right] \right]
\end{aligned}
$$

Here I've brought the $Y$ score inside the summation with a $\frac{1}{c}$ coefficient.

$$
\begin{aligned}
&= \frac{1}{c} \sum^c_{i=1} \left[ n_i r_i \sqrt{\frac{h_i}{h_1}} E \left[    \sum^{m_i} \beta_j G_j \sum^{m_Y} \beta_{jY} G_j \right] \right]
\end{aligned}
$$

And since by equation (7) in power and predicitve accuracy: $ E \left[ \sum^{m_i} \beta_j G_j \sum^{m_Y} \beta_{jY} G_j \right] = m \text{Cov} (\hat{\beta}_i, \beta_Y)$ 

Then
$$Cov(Y, \text{acmPRS}) = \frac{1}{c} \sum^c_{i=1} n_i r_i \sqrt{\frac{h_i}{h_1}} m_i Cov(\hat{\beta}_i, \beta_{Y})$$

\end{proof}

\newpage

\begin{theorem}
$R^2_{Y, \text{acmPRS}} = \frac{ \frac{1}{c} \sum^c_{i=1} n_i r_i \sqrt{\frac{h_i}{h_1}} m_i Cov(\hat{\beta}_i, \beta_{Y})}{ \left( \sum^c_{i=1}  \frac{m_i n^2_i r^2_i h_i}{h_1}  Var(\hat{\beta}_i) +  \sum^c_{i \neq j} n_i n_j r_i r_j \sqrt{\frac{h_i h_j}{h^2_1}} Cov(\hat{S}_i, \hat{S}_j)] \right) \left( \sigma^2_{g} + \sigma^2_{e} \right)}$
\end{theorem}

\end{document}

